ArchSem/ISAManip.v
@@ -1,0 +1,160 @@
+(******************************************************************************)
+(*                                ArchSem                                     *)
+(*                                                                            *)
+(*  Copyright (c) 2021                                                        *)
+(*      Thibaut Pérami, University of Cambridge                               *)
+(*      Zonguyan Liu, Aarhus University                                       *)
+(*      Nils Lauermann, University of Cambridge                               *)
+(*      Jean Pichon-Pharabod, University of Cambridge, Aarhus University      *)
+(*      Brian Campbell, University of Edinburgh                               *)
+(*      Alasdair Armstrong, University of Cambridge                           *)
+(*      Ben Simner, University of Cambridge                                   *)
+(*      Peter Sewell, University of Cambridge                                 *)
+(*                                                                            *)
+(*  All files except SailArmInstTypes.v are distributed under the             *)
+(*  license below (BSD-2-Clause). The former is distributed                   *)
+(*  under a mix of BSD-2-Clause and BSD-3-Clause Clear, as described          *)
+(*  in the file header.                                                       *)
+(*                                                                            *)
+(*                                                                            *)
+(*  Redistribution and use in source and binary forms, with or without        *)
+(*  modification, are permitted provided that the following conditions        *)
+(*  are met:                                                                  *)
+(*                                                                            *)
+(*   1. Redistributions of source code must retain the above copyright        *)
+(*      notice, this list of conditions and the following disclaimer.         *)
+(*                                                                            *)
+(*   2. Redistributions in binary form must reproduce the above copyright     *)
+(*      notice, this list of conditions and the following disclaimer in the   *)
+(*      documentation and/or other materials provided with the distribution.  *)
+(*                                                                            *)
+(*  THIS SOFTWARE IS PROVIDED BY THE COPYRIGHT HOLDERS AND CONTRIBUTORS       *)
+(*  "AS IS" AND ANY EXPRESS OR IMPLIED WARRANTIES, INCLUDING, BUT NOT         *)
+(*  LIMITED TO, THE IMPLIED WARRANTIES OF MERCHANTABILITY AND FITNESS         *)
+(*  FOR A PARTICULAR PURPOSE ARE DISCLAIMED. IN NO EVENT SHALL THE            *)
+(*  COPYRIGHT HOLDER OR CONTRIBUTORS BE LIABLE FOR ANY DIRECT, INDIRECT,      *)
+(*  INCIDENTAL, SPECIAL, EXEMPLARY, OR CONSEQUENTIAL DAMAGES (INCLUDING,      *)
+(*  BUT NOT LIMITED TO, PROCUREMENT OF SUBSTITUTE GOODS OR SERVICES; LOSS     *)
+(*  OF USE, DATA, OR PROFITS; OR BUSINESS INTERRUPTION) HOWEVER CAUSED AND    *)
+(*  ON ANY THEORY OF LIABILITY, WHETHER IN CONTRACT, STRICT LIABILITY, OR     *)
+(*  TORT (INCLUDING NEGLIGENCE OR OTHERWISE) ARISING IN ANY WAY OUT OF THE    *)
+(*  USE OF THIS SOFTWARE, EVEN IF ADVISED OF THE POSSIBILITY OF SUCH DAMAGE.  *)
+(*                                                                            *)
+(******************************************************************************)
+
+Require Import Strings.String.
+
+Require Import ASCommon.Options.
+Require Import ASCommon.Common.
+Require Import ASCommon.Exec.
+Require Import ASCommon.FMon.
+Require Import ASCommon.StateT.
+
+#[local] Open Scope Z_scope.
+#[local] Open Scope stdpp_scope.
+
+Require Import Interface.
+Require Import TermModels.
+
+
+(** This module define helper function to manipulate ISA models. *)
+Module ISAManip (IWA : InterfaceWithArch) (TM : TermModelsT IWA). (* to be imported *)
+  Import IWA.Arch.
+  Import IWA.Interface.
+  Import TM.
+
+  (** A global variable is a register that is always written before being read.
+      This means it is never used for inter-instruction communication, and can
+      therefore be safely be internalized in the instruction semantics.
+
+      [remove_global_vars] takes the list of global variables to remove. It will
+      crash if one of them is not a global variable, aka it is read before being
+      written *)
+
+  Section GlobalVars.
+    Context (global_vars : gset reg).
+
+    Equations remove_global_vars_handler :
+      fHandler outcome (stateT registerMap iMon) :=
+      remove_global_vars_handler (RegRead reg racc) :=
+        if decide (reg ∈ global_vars) then
+          entry ← mget (dmap_lookup reg);
+          othrow
+            ("Reading global variable " ++ pretty reg ++ " before writing it")%string
+            entry
+        else mcall (RegRead reg racc);
+      remove_global_vars_handler (RegWrite reg racc rv) :=
+        if decide (reg ∈ global_vars) then
+          mSet (dmap_insert reg rv)
+        else mcall (RegWrite reg racc rv);
+      remove_global_vars_handler call := mcall call.
+
+    Definition remove_global_vars `(isem : iMon A) : iMon A :=
+      cinterp remove_global_vars_handler isem ∅ |$> snd.
+
+    Definition remove_global_vars_trace_end `(itrce : fTraceEnd outcome A) : fTraceEnd outcome A :=
+      match itrce with
+      | FTEStop (RegRead reg _) => if decide (reg ∈ global_vars) then FTENothing else itrce
+      | FTEStop (RegWrite reg _ _) => if decide (reg ∈ global_vars) then FTENothing else itrce
+      | _ => itrce
+      end.
+
+    Definition remove_global_vars_traces `(itrc : iTrace A) : iTrace A :=
+      (filter (λ ev, ¬ (is_reg_eventP (λ reg _ _, reg ∈ global_vars) ev)) itrc.1,
+        remove_global_vars_trace_end itrc.2).
+
+    Fixpoint global_vars_consistent_aux (itrc : list iEvent) (r : registerMap) :=
+      match itrc with
+      | RegRead reg _ &→ rv :: tl =>
+          (reg ∈ global_vars → r !d! reg = Some rv) ∧ global_vars_consistent_aux tl r
+      | RegWrite reg _ rv &→ _ :: tl =>
+          global_vars_consistent_aux tl (if decide (reg ∈ global_vars) then dmap_insert reg rv r else r)
+      | _ :: tl => global_vars_consistent_aux tl r
+      | [] => True
+      end.
+
+    Instance global_vars_consistent_aux_dec itrc r :
+      Decision (global_vars_consistent_aux itrc r).
+    Proof. induction itrc as [? | [[] ?]] in r |- *; solve_decision. Defined.
+
+    Definition global_vars_consistent `(itrc : iTrace A) :=
+      global_vars_consistent_aux itrc.1 ∅.
+    Instance global_vars_consistent_dec `(itrc : iTrace A) :
+      Decision (global_vars_consistent itrc) := ltac:(unfold_decide).
+
+
+    (* TODO automate using autorewrite in CDestruct rather than adding this *)
+    #[local] Hint Extern 5 (CDestrSimpl _ ?P _) =>
+      match P with
+      | context [remove_global_vars_handler] =>
+          constructor;
+          progress (autorewrite with remove_global_vars_handler);
+          reflexivity
+      end : typeclass_instances.
+
+    Arguments mget : simpl never.
+
+    Lemma remove_global_vars_equiv `(isem : iMon A) (itrc : iTrace A) :
+      global_vars_consistent itrc →
+      cmatch isem itrc →
+      cmatch (remove_global_vars isem) (remove_global_vars_traces itrc).
+    Proof.
+      destruct itrc as [trc trce].
+      unfold remove_global_vars, cinterp, remove_global_vars_traces.
+      cbn.
+      generalize (∅ : registerMap) as rg.
+      induction isem as [|[[]|[]]] in trc,trce |- * ; intros rg GVC.
+      all: sinv 1.
+      all: deintros.
+      all: cdestruct |- *** #CDestrMatch.
+      all: try econstructor.
+      all: try naive_solver.
+      rewrite ?unfold_stateT_bind.
+      rewrite unfold_stateT_mget.
+      unfold othrow.
+      cdestruct |- *** #CDestrMatch #CDestrEqOpt.
+      naive_solver.
+    Qed.
+  End GlobalVars.
+
+End ISAManip.
